More sharing of definition

code/streaming/Hacl.Streaming.Lemmas.fsti
@@ -8,20 +8,6 @@ open FStar.Mul
 let uint8 = Lib.IntTypes.uint8
 
 #set-options "--fuel 0 --ifuel 0"
-let update_full #a
-  (block_length:pos)
-  (update: a -> (s:S.seq uint8 { S.length s = block_length }) -> a)
-  (update_last: a -> (s:S.seq uint8 { S.length s < block_length }) -> a)
-  (acc: a)
-  (input: S.seq uint8)
-=
-  let n_blocks = S.length input / block_length in
-  let blocks, rest = S.split input (n_blocks * block_length) in
-  assert (S.length rest = S.length input % block_length);
-  Math.Lemmas.multiple_modulo_lemma n_blocks block_length;
-  assert (S.length blocks % block_length = 0);
-  assert (S.length rest < block_length);
-  update_last (mk_update_multi block_length update acc blocks) rest
 
 /// Some helpers to flip the order of arguments
 let repeat_f #a (block_length:pos { block_length < pow2 32 })
@@ -61,7 +47,7 @@ val update_full_is_repeat_blocks:
       let repeat_l = repeat_l block_length update_last input' in
 
       Lib.Sequence.repeat_blocks #uint8 block_length input repeat_f repeat_l acc ==
-      update_full block_length update update_last acc input))
+      Lib.UpdateMulti.update_full block_length update update_last acc input))
     (decreases (S.length input))
 
 open Lib.IntTypes
